templateCoqMisc.v
@@ -1355,10 +1355,8 @@ Definition flattenHeadApp (f: STerm)  : STerm :=
   Definition mkUnknown (s:ident) : STerm := oterm (CUnknown s) [].
 
   Definition totalPiHalfGood_ref : ident  :=  "ReflParam.PiTypeR.totalPiHalfGood".
+  Definition totalPiHalfGood21_ref : ident  :=  "ReflParam.PiTypeR.totalPiHalfGood21".
   Definition RPiS_ref : ident  :=  "ReflParam.common.R_PiS".
   
   Definition mkRPiS (A1 A2 AR B1 B2 BR: STerm) :=
     mkConstApp RPiS_ref [A1;A2;AR;B1;B2;BR].
-
-  Definition mkTotalPiHalfGood (A1 A2 AR B1 B2 BR BtotHalf: STerm) :=
-    mkConstApp totalPiHalfGood_ref [A1;A2;AR;B1;B2;BR;BtotHalf].
